backup

EC/passCertRPG_jazz_proof.ec
@@ -1,10 +1,11 @@
-require import AllCore Distr List PassCertGenerator_jazz.
+require import AllCore Distr List PassCertRPG_jazz.
 from Jasmin require import JModel.
 require RPGTh.
 
 clone include RPGTh.
 
 abbrev EqWordInt word num = W64.to_uint word = num.
+
 op wordsToPolicy m lengthP lowercaseP uppercaseP numbersP specialP : policy =
   {|length=lengthP;
     lowercaseMin=W64.to_uint (loadW64 m (W64.to_uint lowercaseP));
@@ -17,13 +18,57 @@ op wordsToPolicy m lengthP lowercaseP uppercaseP numbersP specialP : policy =
     specialMax=W64.to_uint (loadW64 m (W64.to_uint (specialP + W64.of_int 8)));|}.
 
 
+
 module ConcreteScheme : RPG_T = {
-  generate_password
+
+  var globalMem : global_mem_t
+  var lowercaseAddr, uppercaseAddr, numbersAddr, specialAddr, outputAddr : W64.t
+
+  proc policyToMem(policy:policy) = {
+    globalMem <- storeW64 globalMem (W64.to_uint lowercaseAddr) (W64.of_int policy.`lowercaseMin);
+    globalMem <- storeW64 globalMem (W64.to_uint (lowercaseAddr + (W64.of_int 8)))
+                 (W64.of_int policy.`lowercaseMax);
+    globalMem <- storeW64 globalMem (W64.to_uint uppercaseAddr) (W64.of_int policy.`uppercaseMin);
+    globalMem <- storeW64 globalMem (W64.to_uint (uppercaseAddr + (W64.of_int 8)))
+                 (W64.of_int policy.`uppercaseMax);
+    globalMem <- storeW64 globalMem (W64.to_uint numbersAddr) (W64.of_int policy.`numbersMin);
+    globalMem <- storeW64 globalMem (W64.to_uint (numbersAddr + (W64.of_int 8)))
+                 (W64.of_int policy.`numbersMax);
+    globalMem <- storeW64 globalMem (W64.to_uint specialAddr) (W64.of_int policy.`specialMin);
+    globalMem <- storeW64 globalMem (W64.to_uint (specialAddr + (W64.of_int 8)))
+                 (W64.of_int policy.`specialMax);
+  }
+
+  proc generate_password(policy:policy) : password option = {
+
+    var feedback : W64.t;
+    var output : password option;
+
+    lowercaseAddr <- W64.of_int 0;
+    uppercaseAddr <- W64.of_int 200;
+    numbersAddr <- W64.of_int 400;
+    specialAddr <- W64.of_int 600;
+    outputAddr <- W64.of_int 800;
+
+    policyToMem(policy);
+    
+    feedback <- M.generate_password(W64.of_int policy.`length, lowercaseAddr, uppercaseAddr,
+                                  numbersAddr, specialAddr, outputAddr);
+
+    if (W64.to_uint feedback < 0) {
+      output <- None;
+    } else {
+      
+    }
+
+    return output;
+
+
+  }
+
 }.
 
-lemma concrete_rpg_correctness &m (length:W64.t, lowercase_policies:W64.t,
-                                   uppercase_policies:W64.t, numbers_policies:W64.t,
-                                   special_policies:W64.t, p_output:W64.t) :
-  Pr[Correctness(ConcreteScheme).main(wordsToPolicy m length lowercase_policies uppercase_policies
-                              numbers_policies special_policies) @ &m : res] = 1%r.
+
+lemma concrete_rpg_correctness &m policy :
+  Pr[Correctness(ConcreteScheme).main(policy) @ &m : res] = 1%r.
 proof.
