EC/passCertRPG_jazz.ec
@@ -4,7 +4,7 @@ from Jasmin require import JModel.
 require import Array76.
 require import WArray76.
 
-op [full uniform] RDRAND: W64.t distr.
+op [full uniform] RDRAND: W64.t distr.  
 
 module M = {
   proc rng (range:W64.t) : W64.t = {
